coq-formalisations/FullProduct/SelfComp.v
@@ -1,0 +1,98 @@
+Require Import ssreflect ssrfun ssrbool eqtype ssrnat seq tuple fintype.
+Require Import ZArith zint.
+Require Export Setoid Relation_Definitions.
+
+Require Import WhileLang TrfState.
+
+Set Implicit Arguments.
+Unset Strict Implicit.
+Unset Printing Implicit Defensive.
+
+Definition ident := positive.
+
+Open Scope Z_scope.
+
+
+
+
+Section SCtrf.
+
+Variable ops: opSig.
+
+Variable lFun : LeakFun ops.
+
+Definition ok: ident := xH.
+Definition okSC: ident := xO xH.
+Definition cL: ident := xI xH.
+Definition cR: ident := xO (xO xH).
+Definition leakL: ident := xH.
+(* obs: uma alternativa era registar toda a informação SC no array
+    leak[0] = ok
+    leak[1] = countL
+    leak[2] = countR
+    leak[3..] = leakage...
+PARECE BOA IDEIA!!! :-)
+*)
+
+
+Parameter regLeak : expr ops -> cmd ops.
+Parameter chkLeak : expr ops -> cmd ops.
+Parameter initSC: cmd ops.
+Parameter chkSC: cmd ops.
+
+Parameter  preleak: expr ops -> seq (expr ops).
+Parameter expr_i: bool -> expr ops -> expr ops.
+Parameter lvalue_i: bool -> lvalue ops -> lvalue ops.
+
+Fixpoint procLeak (side:bool) (l: seq (expr ops)) : cmd ops :=
+ match l, side with
+ | [::], _ => @Skip ops
+ | e::es, false => Seq (regLeak e) (procLeak side es)
+ | e::es, true => Seq (chkLeak e) (procLeak side es)
+ end.
+
+Fixpoint mirror (side:bool) (c: cmd ops) {struct c} : cmd ops :=
+ match c with
+ | Skip => @Skip ops
+ | Assert e => Assert (expr_i side e)
+ | Assume e => Assume (expr_i side e)
+ | Assign x e => Seq (Seq (procLeak side (preleak (expr_i side (ValOf x))))
+                          (procLeak side (preleak (expr_i side e))))
+                     (Assign (lvalue_i side x) (expr_i side e))
+ | Seq c1 c2 => Seq (mirror side c1) (mirror side c2)
+ | If b c1 c2 => Seq (Seq (procLeak side (preleak (expr_i side b)))
+                          (procLeak side [:: expr_i side b]))
+                     (If (expr_i side b) (mirror side c1) (mirror side c2))
+ | While b c1 =>
+    Seq (Seq (procLeak side (preleak (expr_i side b)))
+             (procLeak side [:: expr_i side b]))
+        (While (expr_i side b) 
+               (Seq (mirror side c1)
+                    (Seq (procLeak side (preleak (expr_i side b)))
+                         (procLeak side [:: expr_i side b]))))
+ end.
+                 
+Definition selfComp (c: cmd ops) : cmd ops :=
+ (Seq (Seq initSC (Seq (mirror false c) (mirror true c))) chkSC).
+
+Parameter cmd_i: bool -> cmd ops -> cmd ops.
+
+
+Theorem selfComp_A: forall (c:cmd ops) ts1 ts2 (s11 s12 s21 s22: State) l1 l2 l',
+ eval_cmd lFun s11 c l1 (Some s21) ->
+ eval_cmd lFun s12 c l2 (Some s22) ->
+ eval_cmd lFun (joinState ts1 s11 s12) (selfComp c) l' (Some (joinState ts2 s21 s22))
+ /\ l1==l2 = true (* ts2[okSC] /\ ok1 = ok2 *).
+Admitted.
+
+Theorem selfComp_B: forall (c:cmd ops) ts1 ts2 (s11 s12 s21 s22: State) l1 l2 l',
+ eval_cmd lFun (joinState ts1 s11 s12) (selfComp c) l' (Some (joinState ts2 s21 s22)) ->
+ eval_cmd lFun s11 c l1 (Some s21) /\
+ eval_cmd lFun s12 c l2 (Some s22) /\
+ True (* ts2[okSC] = l1==l2 /\ ok1 = ok2 *).
+Admitted.
+
+
+
+End SCtrf.
+
