coq-formalisations/FullProduct/TrfState.v
@@ -1,0 +1,439 @@
+Require Import ssreflect ssrfun ssrbool eqtype ssrnat seq tuple fintype.
+Require Import ZArith zint.
+Require Export Setoid Relation_Definitions.
+
+Require Import WhileLang.
+
+Set Implicit Arguments.
+Unset Strict Implicit.
+Unset Printing Implicit Defensive.
+
+Definition ident := positive.
+
+Open Scope Z_scope.
+
+(** * Combined State
+
+   The product construction demands fresh variables 
+*)
+
+Record trfState := mkTrfSt { ok : Z
+                           ; sc: Z -> Z }.
+
+Definition eqtrfstate (ssa ssb:trfState) : Prop :=
+ ok ssa = ok ssb /\ forall i, sc ssa i = sc ssb i.
+
+Lemma eqtrfstate_refl: forall ss, eqtrfstate ss ss.
+Proof. rewrite /eqtrfstate; move => [s1 s2] /=; split; reflexivity. Qed.
+
+Lemma eqtrfstate_sym: forall ss1 ss2,
+ eqtrfstate ss1 ss2 -> eqtrfstate ss2 ss1.
+Proof.
+by rewrite /eqtrfstate; move => [s11 s12] [s21 s22] /= [-> H]; split.
+Qed.
+
+Lemma eqtrfstate_trans: forall ss1 ss2 ss3,
+ eqtrfstate ss1 ss2 -> eqtrfstate ss2 ss3 -> eqtrfstate ss1 ss3.
+Proof.
+rewrite /eqtrfstate.
+move => [s11 s12] [s21 s22] [s31 s32] /= [-> H1] [-> H2]; split => //.
+by move => i; rewrite (H1 i).
+Qed.
+
+Add Parametric Relation : (trfState) eqtrfstate
+ reflexivity proved by eqtrfstate_refl
+ symmetry proved by eqtrfstate_sym
+ transitivity proved by eqtrfstate_trans
+ as eqtrfstate_equiv.
+
+Definition eqstatePair (ssa ssb:State*State) : Prop :=
+ eqstate ssa.1 ssb.1 /\ eqstate ssa.2 ssb.2.
+
+Lemma eqstatePair_refl: forall ss, eqstatePair ss ss.
+Proof. rewrite /eqstatePair; move => [s1 s2] /=; split; reflexivity. Qed.
+
+Lemma eqstatePair_sym: forall ss1 ss2,
+ eqstatePair ss1 ss2 -> eqstatePair ss2 ss1.
+Proof.
+by rewrite /eqstatePair; move => [s11 s12] [s21 s22] /= [-> ->]; split.
+Qed.
+
+Lemma eqstatePair_trans: forall ss1 ss2 ss3,
+ eqstatePair ss1 ss2 -> eqstatePair ss2 ss3 -> eqstatePair ss1 ss3.
+Proof.
+rewrite /eqstatePair.
+by move => [s11 s12] [s21 s22] [s31 s32] /= [-> ->] [-> ->]; split.
+Qed.
+
+Add Parametric Relation : (State*State) eqstatePair
+ reflexivity proved by eqstatePair_refl
+ symmetry proved by eqstatePair_sym
+ transitivity proved by eqstatePair_trans
+ as eqstatePair_equiv.
+
+Definition eqstateTriple (ssa ssb:State*State*trfState) : Prop :=
+ eqstatePair ssa.1 ssb.1 /\ eqtrfstate ssa.2 ssb.2.
+
+Lemma eqstateTriple_refl: forall ss, eqstateTriple ss ss.
+Proof. by rewrite /eqstateTriple; move => [s1 s2] /=; split. Qed.
+
+Lemma eqstateTriple_sym: forall ss1 ss2,
+ eqstateTriple ss1 ss2 -> eqstateTriple ss2 ss1.
+Proof.
+rewrite /eqstateTriple; move => [s11 s12] [s21 s22] /= [H1 H2]; split.
+ by apply eqstatePair_sym.
+by apply eqtrfstate_sym.
+Qed.
+
+Lemma eqstateTriple_trans: forall ss1 ss2 ss3,
+ eqstateTriple ss1 ss2 -> eqstateTriple ss2 ss3 -> eqstateTriple ss1 ss3.
+Proof.
+rewrite /eqstateTriple.
+move => [[s11 s12] s13] [[s21 s22] s23] [[s31 s32] s33] /=.
+move => [H11 H12] [H21 H22]; split.
+ by eapply eqstatePair_trans; eauto.
+by eapply eqtrfstate_trans; eauto.
+Qed.
+
+Add Parametric Relation : (State*State*trfState) eqstateTriple
+ reflexivity proved by eqstateTriple_refl
+ symmetry proved by eqstateTriple_sym
+ transitivity proved by eqstateTriple_trans
+ as eqstateTriple_equiv.
+
+Add Parametric Morphism : (@fst State State)
+ with signature eqstatePair ==> eqstate
+ as fstState_morph.
+Proof. 
+by rewrite /eqstatePair; move => [s11 s12] [s21 s22] /= [-> _].
+Qed.
+
+Add Parametric Morphism : (@snd State State)
+ with signature eqstatePair ==> eqstate
+ as sndState_morph.
+Proof. 
+by rewrite /eqstatePair; move => [s11 s12] [s21 s22] /= [_ ->].
+Qed.
+
+Add Parametric Morphism : (@fst (State*State) trfState)
+ with signature eqstateTriple ==> eqstatePair
+ as fstStateTriple_morph.
+Proof. 
+by rewrite /eqstateTriple; move => [s11 s12] [s21 s22] /= [-> _].
+Qed.
+
+Add Parametric Morphism : (@snd (State*State) trfState)
+ with signature eqstateTriple ==> eqtrfstate
+ as sndStateTriple_morph.
+Proof. 
+by rewrite /eqstateTriple; move => [s11 s12] [s21 s22] /= [_ H].
+Qed.
+
+Section StateJoin.
+
+Definition idA (f:ident->ident) (i:ident*Z) : ident*Z := (f i.1, i.2).
+
+(** a bijection between [Z+Z] and [Z]                     *)
+Definition id_i1 x := xO x.
+Definition id_i2 x := xI x.
+
+Lemma id_i1_Nodd: forall x y, xI x == id_i1 y = false.
+Proof. move => x y; apply/negP => /eqP H; discriminate H. Qed.
+
+Lemma id_i2_Neven: forall x y, xO x == id_i2 y = false.
+Proof. move => x [y|y|]; apply/negP => /eqP H; discriminate H. Qed.
+
+Definition id_sel x (f1 f2:ident -> Z) (i:ident) : Z :=
+ match i with
+ | xO i' => f1 i'
+ | xI i' => f2 i'
+ | xH => x
+ end.
+Definition id_selA fx (f1 f2:ident*Z -> Z) (i:ident*Z) : Z :=
+ match i.1 with
+ | xO i' => f1 (i',i.2)
+ | xI i' => f2 (i',i.2)
+ | xH => fx i.2
+ end.
+
+(*
+Lemma id_sel_i2: forall z (f1 f2:ident -> Z) (x:ident),
+ id_sel z f1 f2 (id_i2 x) = f2 x.
+Proof. by []. Qed.
+
+Lemma id_selA_i2: forall f1 f2 x z,
+ id_selA f1 f2 (id_i2 x,z) = f2 (x,z).
+Proof.
+move => f1 f2 [x|x|] //= z.
+by rewrite /id_selA /= Pos.succ_pred_double.
+Qed.
+*)
+
+Definition joinState (st: trfState) (s1 s2:State) : State :=
+ (id_sel (ok st) s1.1 s2.1, id_selA (sc st) s1.2 s2.2).
+
+Definition splitState (s:State) : State*State*trfState :=
+ ( (fun i => s.1 (id_i1 i), fun ai => s.2 (idA id_i1 ai))
+ , (fun i => s.1 (id_i2 i), fun ai => s.2 (idA id_i2 ai))
+ , mkTrfSt (s.1 xH) (fun i=>s.2 (xH,i)) ).
+
+Lemma split_joinState_1: forall ts st1 st2,
+ eqstate (splitState (joinState ts st1 st2)).1.1 st1.
+Proof. by []. Qed.
+
+Lemma split_joinState_2: forall ts st1 st2,
+ eqstate (splitState (joinState ts st1 st2)).1.2 st2.
+Proof. by []. Qed.
+
+Lemma join_splitState: forall st,
+ eqstate (joinState (splitState st).2 (splitState st).1.1 (splitState st).1.2) st.
+Proof. move => st [i|i|] => //=.
+Qed.
+
+Definition joinStateEqLow (lowMap:VarRestr) (s:State) : Prop :=
+ eqstateR lowMap (splitState s).1.1 (splitState s).1.2.
+
+Lemma joinState_compat: forall s s',
+ eqtrfstate s s' -> forall st1 st1', 
+ eqstate st1 st1' -> forall st2 st2',
+ eqstate st2 st2' -> eqstate (joinState s st1 st2) (joinState s' st1' st2').
+Proof.
+move => s s' Es st1 st1' EqS1 st2 st2' EqS2 [x|x|] /=.
+  by move: {EqS2} (EqS2 x) => [Es21 Es22]; split.
+ by move: {EqS1} (EqS1 x) => [Es11 Es12]; split.
+move: Es => [/eqP Es1 Es2]; split => //=.
+by move => x; rewrite /id_selA (Es2 x).
+Qed.
+
+Lemma splitState_compat1: forall st st', 
+ eqstate st st' -> eqstate (splitState st).1.1 (splitState st').1.1.
+Proof.
+rewrite /splitState => st st' EqS i /=.
+by move: {EqS} (EqS (id_i1 i)) => [H1 H2]; split.
+Qed.
+
+Lemma splitState_compat2: forall st st', 
+ eqstate st st' -> eqstate (splitState st).1.2 (splitState st').1.2.
+Proof.
+rewrite /splitState => st st' EqS i /=.
+by move: {EqS} (EqS (id_i2 i)) => [H1 H2]; split.
+Qed.
+
+Lemma splitState_compat3: forall st st', 
+ eqstate st st' -> eqtrfstate (splitState st).2 (splitState st').2.
+Proof.
+rewrite /splitState /eqtrfstate => st st' EqS /=.
+move: {EqS} (EqS xH) => [/eqP H1 H2]; split => // i.
+by move: (H2 i) => /eqP ->.
+Qed.
+
+Variable ops: opSig.
+
+Fixpoint ren_expr f (e: expr ops) : expr ops :=
+ match e with
+ | ValOf l => ValOf (ren_lvalue f l)
+ | Const z => @Const ops z
+ | Minus e1 e2 => Minus (ren_expr f e1) (ren_expr f e2)
+ | Mult e1 e2 => Mult (ren_expr f e1) (ren_expr f e2)
+ | Equal e1 e2 => Equal (ren_expr f e1) (ren_expr f e2)
+ | Op o args => @Op ops _ (@ren_texpr f (op_arity o) args)
+ end
+with ren_texpr f {n:nat} (x:texpr ops n) : texpr ops n :=
+ match x with
+ | t_nil => @t_nil ops
+ | t_cons _ x l => t_cons (ren_expr f x) (ren_texpr f l)
+ end
+with ren_lvalue f l :=
+ match l with
+ | Var v => @Var _ (f v)
+ | ArrCell a e => ArrCell (f a) (ren_expr f e)
+ end.
+
+Lemma ren_Minus: forall f (e1 e2:expr ops),
+ ren_expr f (Minus e1 e2) = Minus (ren_expr f e1) (ren_expr f e2).
+Proof. by []. Qed.
+
+Lemma ren_Mult: forall f (e1 e2:expr ops),
+ ren_expr f (Mult e1 e2) = Mult (ren_expr f e1) (ren_expr f e2).
+Proof. by []. Qed.
+
+Lemma ren_Equal: forall f (e1 e2:expr ops),
+ ren_expr f (Equal e1 e2) = Equal (ren_expr f e1) (ren_expr f e2).
+Proof. by []. Qed.
+
+Lemma ren_tcons: forall f (e:expr ops) n (t:texpr ops n),
+ ren_texpr f (t_cons e t) = t_cons (ren_expr f e) (ren_texpr f t).
+Proof. by []. Qed.
+
+Lemma ren_ArrCell: forall f a (e:expr ops),
+ ren_lvalue f (ArrCell a e) = ArrCell (f a) (ren_expr f e).
+Proof. by []. Qed.
+
+Definition expr_i1 e := ren_expr id_i1 e.
+Definition expr_i2 e := ren_expr id_i2 e.
+Definition lvalue_i1 e := ren_lvalue id_i1 e.
+Definition lvalue_i2 e := ren_lvalue id_i2 e.
+
+Lemma eval_expr_join_i1: forall e s st1 st2,
+ eval_expr (joinState s st1 st2) (expr_i1 e) = eval_expr st1 e.
+Proof.
+pose P1 e := (forall s (st1 st2 : State),
+ eval_expr (joinState s st1 st2) (ren_expr xO e) = eval_expr st1 e).
+pose P2 n (args: texpr ops n) := (forall s (st1 st2 : State) zl,
+ eval_texpr (joinState s st1 st2) zl (ren_texpr xO args)
+ = eval_texpr st1 zl args).
+pose P3 l := (forall s (st1 st2 : State),
+ eval_lvalue (joinState s st1 st2) (ren_lvalue xO l) = eval_lvalue st1 l).
+apply (@expr_mixed_ind ops P1 P2 P3); unfold P1, P2, P3.
+(* ValOf *) 
+move => l IH s st1 st2.
+by apply IH.
+(* Const *)
+by move => z s st1 st2 /=.
+(* Minus *)
+move => e1 IH1 e2 IH2 s st1 st2 /=.
+have ->: forall st e1 e2,
+         eval_expr st (Minus e1 e2) = eval_expr st e1 - eval_expr st e2 by [].
+by rewrite IH1 IH2.
+(* Mult *)
+move => e1 IH1 e2 IH2 s st1 st2 /=.
+have ->: forall st e1 e2,
+         eval_expr st (Mult e1 e2) = eval_expr st e1 * eval_expr st e2 by [].
+by rewrite IH1 IH2.
+(* Equal *)
+move => e1 IH1 e2 IH2 s st1 st2 /=.
+have ->: forall st e1 e2,
+         eval_expr st (Equal e1 e2) 
+         = (if eval_expr st e1 == eval_expr st e2 then 1 else 0) by [].
+by rewrite IH1 IH2.
+(* Op *)
+move => o args IH s st1 st2 /=.
+have ->: forall st (args:texpr ops (op_arity o)),
+         eval_expr st (Op args)
+         = op_sem o (eval_texpr st [::] args) by []. 
+by rewrite IH.
+(* t_nil *)
+by move => s st1 st2.
+(* t_cons *)
+move => n e IHe args IHargs s st1 st2 zl /=.
+have E: forall st zl n e (args:texpr ops n),
+         eval_texpr st zl (t_cons e args)
+         = eval_texpr st [:: eval_expr st e & zl] args by [].
+by rewrite !E IHe IHargs.
+(* Var *)
+move => v s st1 st2 /=.
+have E: forall st v,
+         eval_lvalue st (Var ops v)
+         = st.1 v by [].
+by rewrite !E.
+(* ArrCell *)
+move => a i IHi s st1 st2 /=.
+have E: forall st a e,
+         eval_lvalue st (ArrCell a e)
+         = st.2 (a,eval_expr st e) by [].
+by rewrite !E /= /id_selA /= IHi.
+Qed.
+
+Lemma eval_expr_join_i2: forall e s st1 st2,
+ eval_expr (joinState s st1 st2) (expr_i2 e) = eval_expr st2 e.
+Proof.
+pose P1 e := (forall s (st1 st2 : State),
+ eval_expr (joinState s st1 st2) (ren_expr id_i2 e) = eval_expr st2 e).
+pose P2 n (args: texpr ops n) := (forall s (st1 st2 : State) zl,
+ eval_texpr (joinState s st1 st2) zl (ren_texpr id_i2 args)
+ = eval_texpr st2 zl args).
+pose P3 l := (forall s (st1 st2 : State),
+ eval_lvalue (joinState s st1 st2) (ren_lvalue id_i2 l) = eval_lvalue st2 l).
+apply (@expr_mixed_ind ops P1 P2 P3); unfold P1, P2, P3.
+(* ValOf *)
+move => l IH s st1 st2.
+by apply IH.
+(* Const *)
+by move => z s st1 st2 /=.
+(* Minus *)
+move => e1 IH1 e2 IH2 s st1 st2 /=.
+have ->: forall st e1 e2,
+         eval_expr st (Minus e1 e2) = eval_expr st e1 - eval_expr st e2 by [].
+by rewrite IH1 IH2.
+(* Mult *)
+move => e1 IH1 e2 IH2 s st1 st2 /=.
+have ->: forall st e1 e2,
+         eval_expr st (Mult e1 e2) = eval_expr st e1 * eval_expr st e2 by [].
+by rewrite IH1 IH2.
+(* Equal *)
+move => e1 IH1 e2 IH2 s st1 st2 /=.
+have ->: forall st e1 e2,
+         eval_expr st (Equal e1 e2) 
+         = (if eval_expr st e1 == eval_expr st e2 then 1 else 0) by [].
+by rewrite IH1 IH2.
+(* Op *)
+move => o args IH s st1 st2 /=.
+have ->: forall st (args:texpr ops (op_arity o)),
+         eval_expr st (Op args)
+         = op_sem o (eval_texpr st [::] args) by []. 
+by rewrite IH.
+(* t_nil *)
+by move => s st1 st2.
+(* t_cons *)
+move => n e IHe args IHargs s st1 st2 zl /=.
+have E: forall st zl n e (args:texpr ops n),
+         eval_texpr st zl (t_cons e args)
+         = eval_texpr st [:: eval_expr st e & zl] args by [].
+by rewrite !E IHe IHargs.
+(* Var *)
+move => v s st1 st2 /=.
+have E: forall st v,
+         eval_lvalue st (Var ops v)
+         = st.1 v by [].
+by rewrite !E.
+(* ArrCell *)
+move => a i IHi s st1 st2 /=.
+have E: forall st a e,
+         eval_lvalue st (ArrCell a e)
+         = st.2 (a,eval_expr st e) by [].
+by rewrite !E /= IHi /=.
+Qed.
+
+Lemma updLValue_join_i1: forall s st1 st2 x y,
+ eqstate (updLValue (joinState s st1 st2) (lvalue_i1 x) y)
+         (joinState s (updLValue st1 x y) st2).
+Proof.
+move => s st1 st2 [v|a e] y x /=; rewrite /upd; split => //=.
+ move: x => [x|x|] //=.
+ by rewrite id_i1_Nodd.
+move: x => [x|x|] z; rewrite /id_selA xpair_eqE ?id_i1_Nodd //=.
+by rewrite xpair_eqE /id_i1 eval_expr_join_i1.
+Qed.
+Lemma updLValue_join_i2: forall s st1 st2 x y,
+ eqstate (updLValue (joinState s st1 st2) (lvalue_i2 x) y)
+         (joinState s st1 (updLValue st2 x y)).
+Proof.
+move => s st1 st2 [v|a e] y x /=; rewrite /upd; split => //=.
+ move: x => [x|x|] //=.
+ by rewrite id_i2_Neven.
+move: x => [x|x|] z; rewrite /id_selA xpair_eqE ?id_i2_Neven //=.
+by rewrite xpair_eqE /id_i2 eval_expr_join_i2.
+Qed.
+
+Lemma eval_updLValue_i1: forall s st1 st2 x y e,
+ eval_expr (updLValue (joinState s st1 st2) (lvalue_i1 x) y) (expr_i2 e)
+ = eval_expr (joinState s st1 st2) (expr_i2 e).
+Proof. 
+by move=> s st1 st2 x y e; rewrite updLValue_join_i1 !eval_expr_join_i2.
+Qed.
+
+End StateJoin.
+
+Add Parametric Morphism : joinState
+ with signature eqtrfstate ==> eqstate ==> eqstate ==> eqstate
+ as joinState_morph.
+Proof. by intro; apply joinState_compat. Qed.
+
+Add Parametric Morphism : splitState
+ with signature eqstate ==> eqstateTriple
+ as splitState_morph.
+Proof.
+rewrite /eqstateTriple /eqstatePair => s1 s2 EqS.
+by rewrite splitState_compat1 // splitState_compat2 // splitState_compat3.
+Qed.
+
